better naming conventions
thanks https://leanprover.zulipchat.com/#narrow/stream/113489-new-members/topic/.22Program.20Correctness.22.20on.20Computerphile/near/218217170

src/compiler.lean
@@ -3,38 +3,40 @@ import tactic
 namespace compiler
 
 /- expressions are values and add-expressions -/
-inductive expr
-| val : ℕ -> expr
-| add : expr -> expr -> expr
+inductive Expr
+| Val : ℕ -> Expr
+| Add : Expr -> Expr -> Expr
+open Expr
 
 /-- evaluate an expression directly -/
-@[simp] def eval : expr -> ℕ
-| (expr.val n) := n
-| (expr.add a b) := eval a + eval b
+@[simp] def eval : Expr -> ℕ
+| (Val n) := n
+| (Add a b) := eval a + eval b
 
 /-
   we'll compile our expressions to instructions of a stack machine
   which supports push and add operations
 -/
-inductive instr
-| push : ℕ -> instr
-| add : instr
+inductive Instr
+| PUSH : ℕ -> Instr
+| ADD : Instr
+open Instr
 
 /-- execute a list of instructions on a stack -/
-@[simp] def exec : list instr -> list ℕ -> list ℕ
-| ((instr.push n) :: rest) s :=
+@[simp] def exec : list Instr -> list ℕ -> list ℕ
+| ((PUSH n) :: rest) s :=
   exec rest (n :: s)
-| (instr.add :: rest) (a :: b :: s) :=
+| (ADD :: rest) (a :: b :: s) :=
   exec rest ((a + b) :: s)
 | _ s := s
 
 /-- compile an expression to an instruction list -/
-@[simp] def compile : expr -> list instr
-| (expr.val n) := [instr.push n]
-| (expr.add a b) := compile a ++ compile b ++ [instr.add]
+@[simp] def compile : Expr -> list Instr
+| (Val n) := [PUSH n]
+| (Add a b) := compile a ++ compile b ++ [ADD]
 
 /-- compiled expressions only add to the stack when `exec`d -/
-@[simp] lemma exec_compile_concat (e : expr) : ∀ instrs stack,
+@[simp] lemma exec_compile_concat (e : Expr) : ∀ instrs stack,
   exec (compile e ++ instrs) stack = exec instrs (eval e :: stack) :=
 begin
   induction e with n a b iha ihb,
@@ -47,7 +49,7 @@ begin
 end
 
 /-- exec (compile e) = eval e -/
-theorem eval_eq_exec_compile (e : expr) : exec (compile e) [] = [eval e] :=
+theorem eval_eq_exec_compile (e : Expr) : exec (compile e) [] = [eval e] :=
 by simpa using exec_compile_concat e [] []
 
 end compiler
